Linglib.lean
@@ -2969,3 +2969,4 @@ import Linglib.Data.Examples.AlexandropoulouGotzner2024b
 import Linglib.Data.Examples.AlexeyenkoZeijlstra2025
 import Linglib.Data.Examples.Allotey2021
 import Linglib.Data.Examples.AlokBhalla2026
+import Linglib.Data.Examples.AloniVanOrmondt2023
